

# MATH 301 Homework 11

Chris Camano: ccamano@sfsu.edu

4/25/2022

Chapter 10: 2,10,22,30,32,20,42,

## Problem 10.2

Prove that  $1+2+3+4\ldots+n=\frac{n^2+n}{2}$  for all  $n \in \mathbb{Z}^+$

**Proof by induction:**

**Base case:**  $n=3$

$$1 + 2 + 3 = \frac{9 + 3}{2}$$

$$6 = 6$$

**Inductive Hypothesis:**

$$P(k) = \sum_{n=1}^k n = \frac{k^2 + k}{2}$$

**Proving  $P(k+1)$**

$$\begin{aligned} P(k+1) &= \sum_{n=1}^{k+1} n = \frac{(k+1)^2 + k+1}{2} \\ &= \sum_{n=1}^k n + (k+1) = \frac{(k^2 + 3k + 2)}{2} \\ &= \frac{k^2 + k}{2} + (k+1) = \frac{(k^2 + 3k + 2)}{2} \\ \frac{(k^2 + 3k + 2)}{2} &= \frac{(k^2 + 3k + 2)}{2} \end{aligned}$$

It follows that the hypothesis holds for all  $k$  in the positive integers

## Problem 10.10

Prove that  $3|(5^{2n} - 1) \forall n \geq 0, n \in \mathbb{Z}$

**Proof by induction:**

**Base Case:  $n=2$**

$$5^4 - 1 = 624 = 208(3)$$

**Inductive Hypothesis**

$$P(k) = 3|5^{2k} - 1 \therefore 5^{2k} - 1 = 3(x), x \in \mathbb{Z}$$

**Proving  $P(k+1)$**

$$\begin{aligned} P(k+1) &= 5^{2(k+1)} - 1 \\ &= (5^{2k+2}) - 1 \\ &= (5^{2k} 25) - 1 \\ &= 25(5^{2k}) - 1 \\ &= 25(3x + 1) - 1 \\ &= 75x + 24 \\ &= 3(25x + 8) \end{aligned}$$

Therefore it is shown that 3 divides  $P(k+1)$  which implies 3 divides  $P(k)$  for all  $k$

## Problem 10.20

Prove that  $(1 + 2 + 3 + \dots + n)^2 = 1^3 + 2^3 + 3^3 \dots + n^3$

Prove that

$$\left( \sum_{i=1}^n i \right)^2 = \sum_{i=1}^n i^3$$

Recall from problem 10.2 that we proved

$$\sum_{i=1}^n i = \frac{n^2 + n}{2}$$

So we now have to consider:

$$\begin{aligned} \left( \frac{n^2 + n}{2} \right)^2 &= \sum_{i=1}^n i^3 \\ \frac{(n^2 + n)^2}{4} &= \sum_{i=1}^n i^3 \\ \frac{(n^4 + 2n^3 + n^2)}{4} &= \sum_{i=1}^n i^3 \end{aligned}$$

**Poof by induction:**

**Base case:**

let  $n = 3$ :

$$\frac{(3^4 + 2(3^3) + 3^2)}{4} = \sum_{i=1}^3 i^3$$

$$\frac{144}{4} = 1 + 8 + 27$$

$$36 = 36$$

**Inductive hypothesis:**

$$P(k) = \sum_{i=1}^k i^3 = \frac{(k^4 + 2k^3 + k^2)}{4}$$

**Proving  $P(k+1)$**

$$P(k+1) = \sum_{i=1}^{k+1} i^3 = \frac{((k+1)^4 + 2(k+1)^3 + (k+1)^2)}{4}$$

$$P(k+1) = \sum_{i=1}^k i^3 + (k+1)^3 = \frac{(k^4 + 4k^3 + 6k^2 + 4k + 1) + 2(k^3 + 3k^2 + 3k + 1) + (k^2 + 2k + 1)}{4}$$

$$P(k+1) = \sum_{i=1}^k i^3 + (k+1)^3 = \frac{k^4 + 6k^3 + 13k^2 + 12k + 4}{4}$$

$$P(k+1) = \sum_{i=1}^k i^3 + (k+1)^3 = \frac{k^4 + 6k^3 + 13k^2 + 12k + 4}{4}$$

$$P(k+1) = \frac{(k^4 + 2k^3 + k^2)}{4} + (k+1)^3 = \frac{k^4 + 6k^3 + 13k^2 + 12k + 4}{4}$$

$$P(k+1) = \frac{(k^4 + 2k^3 + k^2 + 4((k+1)^3))}{4} = \frac{k^4 + 6k^3 + 13k^2 + 12k + 4}{4}$$

$$P(k+1) = \frac{(k^4 + 2k^3 + k^2 + 4(k^3 + 3k^2 + 3k + 1))}{4} = \frac{k^4 + 6k^3 + 13k^2 + 12k + 4}{4}$$

$$P(k+1) = \frac{k^4 + 6k^3 + 13k^2 + 12k + 4}{4} = \frac{k^4 + 6k^3 + 13k^2 + 12k + 4}{4}$$

Thus it follows by mathematical induction that  $P(k)$  is true for all natural numbers  $n$ .

## Problem 10.22

If  $n \in \mathbb{N}$  then :

$$\prod_{i=1}^n \left[1 - \frac{1}{2^i}\right] \geq \frac{1}{4} + \frac{1}{2^{n+1}}$$

**Proof by induction:**

**Base case:**

Let  $n = 1$ :

$$\begin{aligned}\prod_{i=1}^2 \left[1 - \frac{1}{2^i}\right] &\geq \frac{1}{4} + \frac{1}{2^{2+1}} \\ \left(1 - \frac{1}{2}\right)\left(1 - \frac{1}{2^2}\right) &\geq \frac{1}{4} + \frac{1}{2^3} \\ \frac{3}{8} &\geq \frac{3}{8}\end{aligned}$$

**Inductive Hypothesis**

$$P(k) = \prod_{i=1}^k \left[1 - \frac{1}{2^i}\right] \geq \frac{1}{4} + \frac{1}{2^{k+1}}$$

**Proving  $P(k+1)$**

$$\begin{aligned}P(k+1) &= \prod_{i=1}^{k+1} \left[1 - \frac{1}{2^i}\right] \geq \frac{1}{4} + \frac{1}{2^{k+2}} \\ P(k+1) &= \prod_{i=1}^k \left[1 - \frac{1}{2^i}\right] \left(1 - \frac{1}{2^{k+1}}\right) \geq \frac{1}{4} + \frac{1}{2^{k+2}} \\ \left(\frac{1}{4} + \frac{1}{2^{k+1}}\right) \left(1 - \frac{1}{2^{k+1}}\right) &\geq \frac{1}{4} + \frac{1}{2^{k+2}} \\ \frac{1}{4} - \frac{1}{4(2^{k+1})} + \frac{1}{2^{k+1}} - \frac{1}{2^{k+1}(2^{k+1})} &\geq \frac{1}{4} + \frac{1}{2^{k+2}} \\ \frac{1}{4} - \frac{1}{2^{k+1}} \left(-\frac{1}{4} + 1 - \frac{1}{(2^{k+1})}\right) &\geq \frac{1}{4} + \frac{1}{2^{k+2}} \\ \frac{1}{4} - \frac{1}{2^{k+1}} \left(\frac{3}{4} - \frac{1}{(2^{k+1})}\right) &\geq \frac{1}{4} + \frac{1}{2^{k+2}}\end{aligned}$$

We are proving for values of  $k$  past the base case so we know that  $k$  must be greater than 1  
This implies  $k > 1 \therefore \frac{1}{2^{k+1}} < \frac{1}{2^2}$

Since increasing the exponent of the 2 in the denominator would

lower the value of the rational number, switching the sign and consequently the inequality:

$$\begin{aligned} \frac{1}{2^{k+1}} &< \frac{1}{2^2} = -\frac{1}{2^{k+1}} > -\frac{1}{4} \\ \frac{1}{4} - \frac{1}{2^{k+1}} \left( \frac{3}{4} - \frac{1}{4} \right) &\geq \frac{1}{4} + \frac{1}{2^{k+2}} \\ \frac{1}{4} - \frac{1}{2^{k+1}} \left( \frac{1}{2} \right) &\geq \frac{1}{4} + \frac{1}{2^{k+2}} \\ \frac{1}{4} - \frac{1}{2^{k+2}} &\geq \frac{1}{4} + \frac{1}{2^{k+2}} \end{aligned}$$

Since

**Problem 10.30**

**Problem 10.32**

**Problem 10.42**